Finished proof of evaluation preservation for the const_to_values transformation

erasure/theories/EConstantValues.v
@@ -7,7 +7,7 @@ From MetaRocq.PCUIC Require Import PCUICAstUtils.
 From MetaRocq.Utils Require Import MRList bytestring utils monad_utils.
 From MetaRocq.Erasure Require Import EPrimitive EAst EEnvMap EInduction EGlobalEnv.
 
-
+#[local] Set Default Goal Selector "!".
 Import Kernames.
 Import MonadNotation.
 
@@ -24,7 +24,7 @@ Fixpoint consts_to_values (t : term) : term :=
     (* For now we apply lazy on all constants, wether they already are a value or not *)
   | tConstruct i m args => tConstruct i m (map consts_to_values args)
   | tCase i mch brs =>
-      tCase i mch (map (on_snd consts_to_values) brs)
+      tCase i (consts_to_values mch) (map (on_snd consts_to_values) brs)
   | tFix mfix idx => 
       tFix (map (map_def consts_to_values) mfix) idx
   | tCoFix mfix idx => 
@@ -40,14 +40,16 @@ Fixpoint consts_to_values (t : term) : term :=
 .
 
 Definition consts_to_values_constant_decl (cb : constant_body) : constant_body := 
-  {| cst_body := option_map tLazy cb.(cst_body)|}.
+  {| cst_body := option_map tLazy (option_map consts_to_values cb.(cst_body))|}.
 
-Definition consts_to_values_decl (d : kername * global_decl) : kername * global_decl :=
-  match d.2 with
+
+Definition consts_to_values_global_decl (d : global_decl) : global_decl :=
+  match d with
   | ConstantDecl cb => 
-      (d.1, ConstantDecl (consts_to_values_constant_decl cb))
+      ConstantDecl (consts_to_values_constant_decl cb)
   | InductiveDecl idecl => d
   end.
+Definition consts_to_values_decl (d : kername * global_decl) : kername * global_decl := on_snd consts_to_values_global_decl d.
 
 Definition consts_to_values_env Σ : global_context := 
   List.map consts_to_values_decl Σ.
@@ -62,7 +64,7 @@ From MetaRocq.Common Require Import Transform.
 
 
 
-Lemma is_lambda_consts_to_values (d : def term) :
+Lemma isLambda_consts_to_values (d : def term) :
   isLambda (dbody d) -> isLambda (dbody (map_def consts_to_values d)).
 Proof.
   by destruct d as [? [] ?].
@@ -70,6 +72,7 @@ Qed.
 
 Ltac convert_foralls :=
   repeat match goal with
+  | |- All _ _ => apply Forall_All 
   | H : All _ _ |- _ => apply All_Forall in H
   | H : context[is_true (forallb _ _)] |- _ =>
       rewrite <-forallb_Forall in H
@@ -110,10 +113,10 @@ Proof.
   - intros ? (? & (wf_brs_p & wf_t) &  wf_all);
     rewrite length_map; repeat split; try easy.
     now convert_foralls; simpl.
-  - intros ? [[? is_lambda_all] wf_fix_m]; repeat split.
+  - intros ? [[? isLambda_all] wf_fix_m]; repeat split.
     + assumption.
     + convert_foralls.
-      auto using is_lambda_consts_to_values. 
+      auto using isLambda_consts_to_values. 
     + unfold wf_fix in *.
       rewrite ->andb_and in *.
       destruct wf_fix_m as [? all_wf].
@@ -130,19 +133,16 @@ Proof.
   - intros ? [? h].
     split.
     + destruct p as [? []]; unfold map_prim; simpl; easy.
-    + destruct p as [? []]; unfold map_prim; simpl; [easy..|].
-      inversion X as [| | | ? [h1 h2]]; subst.
+    + inversion X as [| | | ? [h1 h2]]; subst; try easy.
       unfold test_prim, test_array_model in *; simpl in *.
       rewrite ->andb_and in *.
       now convert_foralls.
 Qed.
 
-
-Lemma lookup_inductive_consts_to_values ctx i :
-  lookup_inductive (consts_to_values_env ctx) i = lookup_inductive ctx i.
+Lemma lookup_env_consts_to_values ctx name :
+  lookup_env (consts_to_values_env ctx) name = option_map (consts_to_values_global_decl) (lookup_env ctx name).
 Proof.
   induction ctx as [|[? [|]] ? ?]; simpl; first easy;
-  unfold lookup_inductive, lookup_minductive; simpl;
   repeat (
     match goal with
     | H : context[if ?p then _ else _] |- _ =>
@@ -162,6 +162,15 @@ Proof.
         destruct p eqn:hp
     end; try easy
   ).
+Qed.
+
+
+Lemma lookup_inductive_consts_to_values ctx i :
+  lookup_inductive (consts_to_values_env ctx) i = lookup_inductive ctx i.
+Proof. 
+  unfold lookup_inductive, lookup_minductive; simpl.
+  rewrite lookup_env_consts_to_values.
+  destruct (lookup_env ctx (inductive_mind i)) as [[? | ibody]|]; simpl; reflexivity.
 Qed.
 
 Lemma lookup_constructor_consts_to_values ctx i n :
@@ -245,7 +254,7 @@ Proof.
     + now convert_foralls; simpl.
   - rewrite lookup_projection_consts_to_values.
     now intros ? [[? ?] wf_t]; repeat split.
-  - intros ? [[? is_lambda_all] wf_fix_m]; 
+  - intros ? [[? isLambda_all] wf_fix_m]; 
     repeat split; try assumption.
     unfold wf_fix in *.
     rewrite ->andb_and in *.
@@ -289,10 +298,10 @@ Theorem wf_glob_consts_to_values
   wf_glob (consts_to_values_env ctx).
 Proof.
   induction ctx as [|[? [[[|]]|?]] ? ?];
-  inversion 2; subst; constructor; now rewrite /= ?wf_consts_to_values_env_map_ctx ?fresh_consts_to_values.
+  inversion 2; subst; constructor; now rewrite /= ?wf_consts_to_values_env_map_ctx ?wf_consts_to_values_same_ctx ?fresh_consts_to_values.
 Qed.    
 
-Theorem wf_consts_to_values 
+Theorem wf_consts_to_values
   (efl : EEnvFlags) (flags : WcbvFlags) 
   (input : Transform.program _ term) :
   has_tLazy_Force ->
@@ -308,3 +317,443 @@ Proof.
       wf_consts_to_values_env_map_ctx.
 Qed.
 
+
+Lemma consts_to_values_atom (wfl : WcbvFlags) ctx e :
+  atom (consts_to_values_env ctx) (consts_to_values e) = atom ctx e.
+Proof.
+  destruct e; try (discriminate || easy); simpl.
+  destruct args; simpl; last easy.
+  now rewrite lookup_constructor_consts_to_values.
+Qed.
+
+Lemma consts_to_values_mkApps (e : term) (args : list term) :
+  consts_to_values (mkApps e args) = mkApps (consts_to_values e) (map consts_to_values args).
+Proof.
+  induction args as [| ? ? IH] in e |- *; first reflexivity.
+  rewrite /= IH //.
+Qed.
+
+Lemma mkApps_snoc e args a :
+  tApp (mkApps e args) a = mkApps e (args ++ [a]).
+Proof.
+  induction args in e |- *; easy.
+Qed.
+
+
+Lemma consts_to_values_csubst e1 n e2 :
+  consts_to_values (ECSubst.csubst e1 n e2) =
+  ECSubst.csubst (consts_to_values e1) n (consts_to_values e2).
+Proof.
+  induction e2 using term_forall_list_ind in n, e1 |- *; simpl; try (reflexivity || now f_equal).
+  - destruct (n ?= n0); reflexivity.
+  - f_equal.
+    rewrite !map_map_compose.
+    apply All_map_eq.
+    now convert_foralls.
+  - f_equal.  
+    rewrite !map_map_compose.
+    apply All_map_eq.
+    now convert_foralls.
+  - f_equal; try easy.
+    rewrite !map_map_compose.
+    apply All_map_eq.
+    convert_foralls.
+    intros [names t] hIn; unfold on_snd; simpl in *.
+    now rewrite (X (names, t)).
+  - f_equal.
+    rewrite !map_map_compose.
+    apply All_map_eq.
+    convert_foralls.
+    intros [dname body rarg] hIn; unfold map_def; simpl in *.
+    now rewrite length_map (X _ hIn).
+  - f_equal.
+    rewrite !map_map_compose.
+    apply All_map_eq.
+    convert_foralls.
+    intros [dname body rarg] hIn; unfold map_def; simpl in *.
+    now rewrite length_map (X _ hIn).
+  - f_equal.
+    inversion X as [| | | ? [heq eq_All]]; subst; try reflexivity.
+    rewrite /map_prim /= /map_array_model /= heq.
+    do 3 f_equal.
+    rewrite !map_map_compose.
+    apply All_map_eq.
+    now convert_foralls.
+Qed.
+
+Lemma consts_to_values_substl l e :
+  consts_to_values (ECSubst.substl l e) =
+  ECSubst.substl (map consts_to_values l) (consts_to_values e).
+Proof.
+  induction l as [| ? ? IH] 
+    using list_ind_rev; simpl; first reflexivity.
+  rewrite /ECSubst.substl map_app !fold_left_app.
+  fold (ECSubst.substl l e); simpl.
+  fold (ECSubst.substl (map consts_to_values l) (consts_to_values e)); simpl.
+  now rewrite consts_to_values_csubst IH.
+Qed. 
+
+Lemma map_fix_subst mfix :
+  map consts_to_values (fix_subst mfix) = fix_subst (map (map_def consts_to_values) mfix).
+Proof.
+  unfold fix_subst.
+  rewrite length_map.
+  remember #|mfix| as n eqn:heq.
+  clear heq.
+  induction n as [|? IH]; first reflexivity.
+  rewrite map_cons /=; f_equal.
+  now rewrite IH.
+Qed.
+
+Lemma consts_to_values_cunfold_fix mfix idx :
+  cunfold_fix (map (map_def consts_to_values) mfix) idx =
+  option_map (on_snd consts_to_values) (cunfold_fix mfix idx).
+Proof.
+  unfold cunfold_fix.
+  rewrite nth_error_map.
+  destruct (nth_error mfix idx); unfold on_snd; simpl; last reflexivity.
+  now rewrite consts_to_values_substl map_fix_subst.
+Qed.
+
+Lemma map_cofix_subst mfix :
+  map consts_to_values (cofix_subst mfix) = cofix_subst (map (map_def consts_to_values) mfix).
+Proof.
+  unfold cofix_subst.
+  rewrite length_map.
+  remember #|mfix| as n eqn:heq.
+  clear heq.
+  induction n as [|? IH]; first reflexivity.
+  rewrite map_cons /=; f_equal.
+  now rewrite IH.
+Qed.
+
+Lemma consts_to_values_cunfold_cofix mfix idx :
+  cunfold_cofix (map (map_def consts_to_values) mfix) idx =
+  option_map (on_snd consts_to_values) (cunfold_cofix mfix idx).
+Proof.
+  unfold cunfold_cofix.
+  rewrite nth_error_map.
+  destruct (nth_error mfix idx); unfold on_snd; simpl; last reflexivity.
+  now rewrite consts_to_values_substl map_cofix_subst.
+Qed.
+
+
+
+
+Lemma consts_to_values_ind_isprop_and_pars ctx ind :
+  inductive_isprop_and_pars (consts_to_values_env ctx) ind =
+  inductive_isprop_and_pars ctx ind.
+Proof.
+  rewrite
+    /inductive_isprop_and_pars 
+    lookup_inductive_consts_to_values //.
+Qed.
+Lemma consts_to_values_constr_isprop_pars_decl ctx ind n :
+  constructor_isprop_pars_decl (consts_to_values_env ctx) ind n =
+  constructor_isprop_pars_decl ctx ind n.
+Proof.
+  rewrite
+    /constructor_isprop_pars_decl 
+    lookup_constructor_consts_to_values //.
+Qed.  
+
+
+Lemma consts_to_values_declared_constant ctx c decl :
+  declared_constant ctx c decl ->
+  declared_constant (consts_to_values_env ctx) c (consts_to_values_constant_decl decl).
+Proof.
+  unfold declared_constant.
+  rewrite lookup_env_consts_to_values.
+  destruct (lookup_env ctx c); intros [=->].
+  reflexivity.
+Qed.
+
+Lemma consts_to_values_cst_body  decl :
+  cst_body (consts_to_values_constant_decl decl) = option_map (fun t => tLazy (consts_to_values t)) (cst_body decl). 
+Proof.
+  destruct decl as [[?|]]; reflexivity.
+Qed.
+
+Lemma consts_to_values_head e :
+  EAstUtils.head (consts_to_values e) = consts_to_values (EAstUtils.head e).
+Proof.
+  induction e; simpl; try reflexivity.
+  now rewrite !EAstUtils.head_tApp.
+Qed.  
+
+Lemma consts_to_values_isLambda e : 
+  isLambda (consts_to_values e) = isLambda e.
+Proof.
+  destruct e; reflexivity.
+Qed.
+Lemma consts_to_values_isFixApp e : EAstUtils.isFixApp (consts_to_values e) = EAstUtils.isFixApp e.
+Proof.
+  unfold EAstUtils.isFixApp.
+  rewrite consts_to_values_head.
+  destruct (EAstUtils.head e); reflexivity.
+Qed.
+
+Lemma consts_to_values_isFix e : 
+  EAstUtils.isFix (consts_to_values e) = EAstUtils.isFix e.
+Proof.
+  destruct e; reflexivity.
+Qed.
+
+Lemma consts_to_values_isBox e : EAstUtils.isBox (consts_to_values e) = EAstUtils.isBox e.
+Proof.
+  destruct e; reflexivity.
+Qed.
+
+Lemma consts_to_values_isConstructApp e :
+  EAstUtils.isConstructApp (consts_to_values e) = EAstUtils.isConstructApp e.
+Proof.
+  unfold EAstUtils.isConstructApp.
+  rewrite consts_to_values_head.
+  destruct (EAstUtils.head e); reflexivity.
+Qed.
+
+Lemma consts_to_values_isPrimApp e : EAstUtils.isPrimApp (consts_to_values e) = EAstUtils.isPrimApp e.
+Proof.
+  unfold EAstUtils.isPrimApp.
+  rewrite consts_to_values_head.
+  destruct (EAstUtils.head e); reflexivity.
+Qed.
+
+Lemma consts_to_values_isLazyApp e : EAstUtils.isLazyApp (consts_to_values e) = EAstUtils.isLazyApp e.
+Proof.
+  unfold EAstUtils.isLazyApp.
+  rewrite consts_to_values_head.
+  destruct (EAstUtils.head e); reflexivity.
+Qed.
+
+Lemma consts_to_values_iota pars args br :
+  consts_to_values (iota_red pars args br) = 
+  iota_red 
+    pars 
+    (map consts_to_values args) 
+    (on_snd consts_to_values br).
+Proof.
+  rewrite /iota_red consts_to_values_substl -map_skipn map_rev //.
+Qed.
+
+
+
+#[local] Ltac destruct_IHs :=
+    repeat match goal with 
+    | IH : _ -> 
+      eval (consts_to_values_env _) _ _
+        |- _ =>
+        unshelve epose proof IH _; first try easy;
+        clear IH
+    end;[
+      try solve[
+        repeat match goal with
+        | h : is_true (is_nil ?l) |- _ => 
+            destruct l; last (simpl in h; easy); clear h
+        | h : _ /\ _ |- _ => destruct h
+        | h : is_true (_ && _) |- _ => apply andb_andI in h
+        | h : eval _ _ _ |- _ => 
+            apply eval_wellformed in h; [|easy..]; simpl in h
+        | h : is_true (wellformed _ _ (mkApps _ _)) |- _ =>
+            rewrite wellformed_mkApps /= in h
+        | |- is_true (wellformed _ _ (iota_red _ _ _)) => 
+            eapply wellformed_iota_red_brs
+        | |- is_true (wellformed _ _ (ECSubst.csubst _ _ _)) => 
+            eapply wellformed_csubst
+        | |- context[is_true (_ && _)] => rewrite andb_and
+        | |- _ /\ _ => split; try easy
+        | h : ?P |- ?P => assumption
+        | |- is_true (wellformed _ _ (mkApps _ _)) =>
+            rewrite wellformed_mkApps /=
+        | h : cunfold_fix _ _ = Some (_, ?e) |-
+            is_true (wellformed _ _ ?e) => 
+            eapply wellformed_cunfold_fix; simpl
+        | h : cunfold_cofix _ _ = Some (_, ?e) |-
+            is_true (wellformed _ _ ?e) => 
+            eapply wellformed_cunfold_cofix; simpl
+        | h : nth_error _ _ = Some ?a |-
+              is_true (wellformed _ _ ?a) => eapply nth_error_forallb
+        | h : context[if ?c then _ else _] |- _ => 
+            destruct c eqn:?
+        end; easy
+      ]..
+    |].
+
+Ltac my_simpl :=
+  repeat match goal with
+  | h : nth_error ?l ?n = Some ?r |-
+      nth_error (map _ ?l) ?n = Some _ =>
+        rewrite nth_error_map h //=
+  | |- context[#|map _ _|] => rewrite length_map //
+  | |- context[#|skipn _ (map _ _)|] => rewrite -map_skipn /=
+  end.
+
+
+Theorem trust_consts_to_values_pres :
+  forall (efl : EEnvFlags) (wfl : WcbvFlags) (p : Transform.program _ term)
+  (v : term),
+  has_tApp -> (* Needed for eval_wellformed *)
+  has_tBox -> (*  *)
+  wf_eprogram efl p ->
+  eval_eprogram wfl p v ->
+  let ip := consts_to_values_program p in
+  eval_eprogram wfl ip (consts_to_values v).
+Proof.
+  intros ? ? [ctx e] ? ? htBox [wf_ctx wf_e] [eval_e]; simpl in *.
+  constructor; simpl.
+  induction eval_e; simpl in *; try rewrite ->!andb_and in *.
+  - destruct_IHs. econstructor; eassumption.
+  - destruct_IHs.
+    econstructor; try eassumption.
+    now rewrite -consts_to_values_csubst.
+  - destruct_IHs.
+    econstructor; first eassumption.
+    now rewrite -consts_to_values_csubst.
+  - destruct_IHs.
+    econstructor.
+    + assumption.
+    + now rewrite consts_to_values_mkApps in H1.
+    + rewrite consts_to_values_constr_isprop_pars_decl e1 //.
+    + erewrite nth_error_map, e2; simpl.
+      reflexivity.
+    + rewrite length_map. eassumption. 
+    + rewrite -map_skipn length_map. 
+      destruct br; simpl in *. assumption.
+    + rewrite -consts_to_values_iota //.
+  - destruct_IHs.
+    eapply eval_iota_block.
+    + assumption.
+    + eassumption.
+    + rewrite consts_to_values_constr_isprop_pars_decl e1 //.
+    + my_simpl.
+    + my_simpl.
+    + my_simpl.
+    + rewrite -consts_to_values_iota //.
+  - destruct_IHs.
+    { subst brs. simpl in *.
+      rewrite ->andb_and in *.
+      destruct wf_e as (_ & _ & wf_f4 & _).
+      apply wellformed_substl; last rewrite repeat_length //.
+      remember #|n| as len.
+      move:htBox.
+      clear.
+      induction len; simpl; first easy.
+      rewrite andb_and; split; easy. }
+    eapply eval_iota_sing.
+    + assumption.
+    + assumption.
+    + rewrite consts_to_values_ind_isprop_and_pars //.
+    + subst; reflexivity.
+    + change tBox with (consts_to_values tBox).
+      rewrite -map_repeat -consts_to_values_substl.
+      assumption.
+  - destruct_IHs.
+    eapply eval_fix; simpl in *.
+    + assumption.
+    + now rewrite consts_to_values_mkApps /= in H2.
+    + eassumption.
+    + rewrite consts_to_values_cunfold_fix e1 length_map //.
+    + rewrite -consts_to_values_mkApps //.
+  - destruct_IHs.
+    rewrite consts_to_values_mkApps /=.
+    eapply eval_fix_value.
+    + assumption.
+    + now rewrite consts_to_values_mkApps /= in H1.
+    + eassumption.
+    + rewrite consts_to_values_cunfold_fix e1.
+      reflexivity.
+    + my_simpl.
+  - destruct_IHs.
+    eapply eval_fix'; try eassumption.
+    rewrite consts_to_values_cunfold_fix e0; reflexivity.
+  - destruct_IHs.
+    eapply eval_cofix_case.
+    + rewrite consts_to_values_mkApps /= in H1.
+      eassumption.
+    + rewrite consts_to_values_cunfold_cofix e0 /on_snd //.
+    + rewrite consts_to_values_mkApps // in H0.
+  - destruct_IHs.
+    eapply eval_cofix_proj.
+    + rewrite consts_to_values_mkApps /= in H1.
+      eassumption.
+    + rewrite consts_to_values_cunfold_cofix e0 /on_snd //.
+    + rewrite consts_to_values_mkApps // in H0.
+  - destruct_IHs.
+    { rewrite /lookup_constant isdecl /= in wf_e.
+      apply lookup_env_wellformed in isdecl; last assumption.
+      rewrite /wf_global_decl e //= in isdecl. }
+    eapply eval_force.
+    + econstructor.
+      * now apply consts_to_values_declared_constant. 
+      * rewrite consts_to_values_cst_body e //.
+      * do 2 constructor.
+    + assumption.
+  - destruct_IHs.
+    eapply eval_proj.
+    + assumption.
+    + now rewrite consts_to_values_mkApps in H1.
+    + now rewrite consts_to_values_constr_isprop_pars_decl.
+    + my_simpl.
+    + my_simpl.
+    + assumption. 
+  - destruct_IHs.
+    eapply eval_proj_block.
+    + assumption.
+    + eassumption.
+    + now rewrite consts_to_values_constr_isprop_pars_decl.
+    + my_simpl.
+    + my_simpl.
+    + assumption.
+  - destruct_IHs.
+    apply eval_proj_prop; try assumption.
+    now rewrite consts_to_values_ind_isprop_and_pars.
+  - destruct_IHs.
+    rewrite consts_to_values_mkApps /=.
+    eapply eval_construct.
+    + assumption.
+    + now rewrite lookup_constructor_consts_to_values.
+    + now rewrite consts_to_values_mkApps in H1.
+    + my_simpl.
+    + assumption.
+  - destruct_IHs.
+    eapply eval_construct_block.
+    + assumption.
+    + now rewrite lookup_constructor_consts_to_values.
+    + my_simpl.
+    + destruct cstr_as_blocks; last first.
+      { destruct args; last easy. 
+        inversion a; subst.
+        constructor. }
+      rewrite /lookup_constructor_pars_args e0 /= in wf_e.
+      destruct wf_e as [[? ?] [? ?]%andb_andI].
+      apply All2_All2_Set, All2_map.
+      apply All2_over_undep in iha.
+      unshelve eapply (All2_apply_dep_arrow _ iha).
+      now convert_foralls.
+  - destruct_IHs.
+    apply eval_app_cong; try assumption.
+    rewrite 
+      consts_to_values_isLambda
+      consts_to_values_isFixApp
+      consts_to_values_isFix
+      consts_to_values_isBox
+      consts_to_values_isConstructApp
+      consts_to_values_isPrimApp
+      consts_to_values_isLazyApp
+      //.
+  - inversion X; subst; try solve[repeat constructor].
+    rewrite /test_prim /= /test_array_model /= in wf_e.
+    destruct wf_e as [? [? ?]%andb_andI].
+    destruct_IHs.
+    unfold map_prim; simpl.
+    do 2 constructor; last assumption.
+    subst a a'; simpl in *.
+    apply All2_All2_Set, All2_map.
+    apply All2_over_undep in X0.
+    unshelve eapply (All2_apply_dep_arrow _ X0).
+    now convert_foralls.
+  - destruct_IHs.
+    econstructor; eassumption.
+  - apply eval_atom.
+    now rewrite consts_to_values_atom.
+Qed.
